Fix and prove Is_conv_to_Arity_inv

pcuic/theories/PCUICPrincipality.v
@@ -28,12 +28,23 @@ Section Principality.
   Context (Σ : global_env_ext).
   Context (wfΣ : wf Σ).
 
-  Definition Is_conv_to_Arity Σ Γ T := exists T', ∥red Σ Γ T T'∥ /\ isArity T'.
- 
-  Lemma Is_conv_to_Arity_inv Γ T :
-    Is_conv_to_Arity Σ Γ T ->
-    (exists na A B, ∥red Σ Γ T (tProd na A B)∥) \/ (exists u, ∥red Σ Γ T (tSort u)∥).
-  Admitted.
+  Definition Is_conv_to_Arity Σ Γ T :=
+    exists T', ∥ red Σ Γ T T' ∥ /\ isArity T'.
+
+  Lemma Is_conv_to_Arity_inv :
+    forall Γ T,
+      Is_conv_to_Arity Σ Γ T ->
+      (exists na A B, ∥ red Σ Γ T (tProd na A B) ∥) \/
+      (exists na b B t, ∥ red Σ Γ T (tLetIn na b B t) ∥) \/
+      (exists u, ∥ red Σ Γ T (tSort u) ∥).
+  Proof.
+    intros Γ T [T' [r a]].
+    destruct T'.
+    all: try contradiction.
+    - right. right. eexists. eassumption.
+    - left. eexists _, _, _. eassumption.
+    - right. left. eexists _, _, _, _. eassumption.
+  Qed.
 
   Lemma invert_red_sort Γ u v :
     red Σ Γ (tSort u) v -> v = tSort u.
