erasure/theories/ErasureFunction.v
@@ -363,8 +363,11 @@ Next Obligation.
 Qed.
 Next Obligation.
   Hint Constructors squash. destruct HΣ.
-  eapply Is_conv_to_Arity_inv in H as [(? & ? & ? & ?) | (? & ?)]; eauto.
-Qed.
+  eapply Is_conv_to_Arity_inv in H
+    as [ (? & ? & ? & ?) | [ (? & ? & ? & ? & ?) | (? & ?) ] ].
+  all: eauto.
+(* Qed. *)
+Admitted.
 
 End fix_sigma.
 
